ported Zipperposition loop to new version of DISCOUNT loop

Given_Clause_Loops/Zipperposition_Loop.thy
@@ -1,7 +1,8 @@
 (* Title:        Zipperposition Loop
    Authors:      Qi Qiu, 2021
                  Jasmin Blancherte <j.c.blanchette at vu.nl>, 2022
-   Maintainer:   Sophie Tourret <stourret at loria.fr>, 2021 *)
+   Maintainer:   Sophie Tourret <stourret at loria.fr>, 2021
+*)
 
 section \<open>Zipperposition Loop\<close>
 
@@ -9,40 +10,23 @@ theory Zipperposition_Loop
   imports DISCOUNT_Loop
 begin
 
-locale zipperposition_loop =
-  discount_loop Bot_F Inf_F Bot_G Q entails_q Inf_G_q Red_I_q
-    Red_F_q \<G>_F_q \<G>_I_q Equiv_F Prec_F Prec_L active passive y
-  for
-    Bot_F :: "'f set" and
-    Inf_F :: "'f inference set" and
-    Bot_G :: "'g set" and
-    Q :: "'q set" and
-    entails_q :: "'q \<Rightarrow> 'g set \<Rightarrow> 'g set \<Rightarrow> bool" and
-    Inf_G_q :: \<open>'q \<Rightarrow> 'g inference set\<close> and
-    Red_I_q :: "'q \<Rightarrow> 'g set \<Rightarrow> 'g inference set" and
-    Red_F_q :: "'q \<Rightarrow> 'g set \<Rightarrow> 'g set" and
-    \<G>_F_q :: "'q \<Rightarrow> 'f \<Rightarrow> 'g set" and
-    \<G>_I_q :: "'q \<Rightarrow> 'f inference \<Rightarrow> 'g inference set option" and
-    Equiv_F :: "'f \<Rightarrow> 'f \<Rightarrow> bool" (infix "\<doteq>" 50) and
-    Prec_F :: "'f \<Rightarrow> 'f \<Rightarrow> bool" (infix "\<prec>\<cdot>" 50) and
-    Prec_L :: "'l \<Rightarrow> 'l \<Rightarrow> bool" (infix "\<sqsubset>L" 50) and
-    active passive y :: 'l
+context discount_loop
 begin
 
 
 subsection \<open>Definition and Lemmas\<close>
 
-fun zl_inferences_of :: " ('f inference llist) set \<Rightarrow> 'f inference set " where
+fun zl_inferences_of :: "'f inference llist set \<Rightarrow> 'f inference set " where
   "zl_inferences_of T = \<Union> {lset x |x. x \<in> T}"
 
 fun
   zl_state :: "'f inference llist set \<times> 'f set \<times> 'f set \<times> 'f set \<Rightarrow>
-    'f inference set \<times> ('f \<times> 'l) set"
+    'f inference set \<times> ('f \<times> DL_label) set"
 where
   "zl_state (T, P, Y, A) = (zl_inferences_of T, formulas_of (P, Y, A))"
 
 inductive
-  ZL :: "'f inference set \<times> ('f \<times> 'l) set \<Rightarrow> 'f inference set \<times> ('f \<times> 'l) set \<Rightarrow> bool"
+  ZL :: "'f inference set \<times> ('f \<times> DL_label) set \<Rightarrow> 'f inference set \<times> ('f \<times> DL_label) set \<Rightarrow> bool"
   (infix "\<leadsto>ZL" 50)
 where
   choose_p: "zl_state (T, P \<union> {C}, {}, A) \<leadsto>ZL zl_state (T, P, {C}, A)"
@@ -59,7 +43,7 @@ where
 | schedule_infer: "zl_inferences_of T' = (no_labels.Inf_between A {C}) \<Longrightarrow>
     zl_state (T, P, {C}, A) \<leadsto>ZL zl_state (T \<union> T', P, {}, A \<union> {C})"
 | delete_orphans: "\<forall>n \<in> {n. enat n < llength \<iota>s}. lnth \<iota>s n \<notin> no_labels.Inf_from A \<Longrightarrow>
-    zl_state (T \<union> { \<iota>s }, P, Y, A) \<leadsto>ZL zl_state (T, P, Y, A)"
+    zl_state (T \<union> {\<iota>s}, P, Y, A) \<leadsto>ZL zl_state (T, P, Y, A)"
 
 lemma flatten: " zl_inferences_of {(LCons \<iota>0 \<iota>s)} = zl_inferences_of {\<iota>s} \<union> { \<iota>0 }"
   by auto
@@ -78,11 +62,9 @@ lemma zl_choose_p_in_lgc: "zl_state (T, P \<union> {C}, {}, A) \<leadsto>LGC zl_
 proof -
   let ?\<N> = "formulas_of (P, {}, A)"
   and ?\<T> = "zl_inferences_of T"
-  have "passive \<sqsupset>L y"
-    by (simp add: order_on_labels)
-  moreover have "y \<noteq> active"
-    using labels_distinct by simp
-  ultimately have "(?\<T>, ?\<N> \<union> {(C, passive)}) \<leadsto>LGC (?\<T>, ?\<N> \<union> {(C, y)})"
+  have "Passive \<sqsupset>L YY"
+    by (simp add: DL_Prec_L_def)
+  then have "(?\<T>, ?\<N> \<union> {(C, Passive)}) \<leadsto>LGC (?\<T>, ?\<N> \<union> {(C, YY)})"
     using relabel_inactive by blast
   then have "(?\<T>, formulas_of (P \<union> {C}, {}, A)) \<leadsto>LGC (?\<T>, formulas_of (P, {C}, A))"
      by (metis PYA_add_passive_formula P0A_add_y_formula)
@@ -91,25 +73,25 @@ proof -
 qed
 
 lemma zl_delete_fwd_in_lgc:
-  assumes " (C \<in> no_labels.Red_F A) \<or> (\<exists>C'\<in>A. C' \<preceq>\<cdot> C)"
+  assumes "C \<in> no_labels.Red_F A \<or> (\<exists>C' \<in> A. C' \<preceq>\<cdot> C)"
   shows "zl_state (T, P, {C}, A) \<leadsto>LGC zl_state (T, P, {}, A)"
   using assms
 proof
   assume c_in: "C \<in> no_labels.Red_F A"
-  then have "A \<subseteq> fst ` (formulas_of (P, {}, A))"
+  then have "A \<subseteq> fst ` formulas_of (P, {}, A)"
     by simp
-  then have "C \<in> no_labels.Red_F (fst ` (formulas_of (P, {}, A)))"
+  then have "C \<in> no_labels.Red_F (fst ` formulas_of (P, {}, A))"
     by (metis (no_types, lifting) c_in in_mono no_labels.Red_F_of_subset)
   then show ?thesis
     using remove_redundant_no_label by auto
 next
-  assume "\<exists>C'\<in>A. C' \<preceq>\<cdot> C"
+  assume "\<exists>C' \<in> A. C' \<preceq>\<cdot> C"
   then obtain C' where c'_in_and_c'_ls_c: "C' \<in> A \<and> C' \<preceq>\<cdot> C"
     by auto
-  then have "(C', active) \<in> formulas_of (P, {}, A)"
+  then have "(C', Active) \<in> formulas_of (P, {}, A)"
     by auto
-  moreover have "y \<sqsupset>L active" using order_on_labels
-    by simp
+  moreover have "YY \<sqsupset>L Active"
+    by (simp add: DL_Prec_L_def)
   ultimately show ?thesis
     by (metis P0A_add_y_formula remove_succ_L c'_in_and_c'_ls_c zl_state.simps)
 qed
@@ -119,20 +101,20 @@ lemma zl_simplify_fwd_in_lgc:
   shows "zl_state (T, P, {C}, A) \<leadsto>LGC zl_state (T, P, {C'}, A)"
 proof -
   let ?\<N> = "formulas_of (P, {}, A)"
-  and ?\<M> = "{(C, y)}"
-  and ?\<M>'= "{(C', y)}"
-  have "A \<union> {C'} \<subseteq> fst` (?\<N> \<union> ?\<M>')"
+  and ?\<M> = "{(C, YY)}"
+  and ?\<M>'= "{(C', YY)}"
+  have "A \<union> {C'} \<subseteq> fst ` (?\<N> \<union> ?\<M>')"
     by auto
   then have "C \<in> no_labels.Red_F_\<G> (fst` (?\<N> \<union> ?\<M>'))"
     by (smt (verit, ccfv_SIG) assms no_labels.Red_F_of_subset subset_iff)
-  then have "(C, y) \<in> Red_F (?\<N> \<union> ?\<M>')"
+  then have "(C, YY) \<in> Red_F (?\<N> \<union> ?\<M>')"
     using no_labels_Red_F_imp_Red_F by simp
   then have "?\<M> \<subseteq> Red_F_\<G> (?\<N> \<union> ?\<M>')"
     by simp
   moreover have "active_subset ?\<M>' = {}"
-    using active_subset_def order_on_labels labels_distinct by auto
-  ultimately have "(zl_inferences_of T, formulas_of (P, {}, A) \<union> {(C, y)}) \<leadsto>LGC
-                    (zl_inferences_of T, formulas_of (P, {}, A) \<union> {(C', y)})"
+    using active_subset_def by auto
+  ultimately have "(zl_inferences_of T, formulas_of (P, {}, A) \<union> {(C, YY)}) \<leadsto>LGC
+    (zl_inferences_of T, formulas_of (P, {}, A) \<union> {(C', YY)})"
     using process[of _ _ "?\<M>" _ "?\<M>'"] by auto
   then show ?thesis
     by simp
@@ -150,17 +132,18 @@ proof
     by simp
   then have "C' \<in> no_labels.Red_F_\<G> (fst` ?\<N>)"
     by (metis (no_types, lifting) c'_in insert_Diff insert_subset no_labels.Red_F_of_subset)
-  then have "(zl_inferences_of T, ?\<N> \<union> {(C', active)}) \<leadsto>LGC (zl_inferences_of T, ?\<N>)"
+  then have "(zl_inferences_of T, ?\<N> \<union> {(C', Active)}) \<leadsto>LGC (zl_inferences_of T, ?\<N>)"
     using remove_redundant_no_label by auto
 
-  moreover have "?\<N> \<union> {(C', active)} = formulas_of (P, {C}, A \<union> {C'})"
+  moreover have "?\<N> \<union> {(C', Active)} = formulas_of (P, {C}, A \<union> {C'})"
     using PYA_add_active_formula by blast
-  ultimately have "(zl_inferences_of T, formulas_of (P, {C}, A \<union> {C'})) \<leadsto>LGC zl_state (T, P, {C}, A)"
+  ultimately have "(zl_inferences_of T, formulas_of (P, {C}, A \<union> {C'})) \<leadsto>LGC
+    zl_state (T, P, {C}, A)"
     by simp
   then show ?thesis by auto
 next
   assume "C' \<cdot>\<succ> C"
-  moreover have "(C, y) \<in> formulas_of (P, {C}, A)"
+  moreover have "(C, YY) \<in> formulas_of (P, {C}, A)"
     by simp
   ultimately show ?thesis
     by (metis remove_succ_F PYA_add_active_formula zl_state.simps)
@@ -170,8 +153,8 @@ lemma zl_simplify_bwd_in_lgc:
   assumes "C' \<in> no_labels.Red_F_\<G> {C, C''}"
   shows "zl_state (T, P, {C}, A \<union> {C'}) \<leadsto>LGC zl_state (T, P \<union> {C''}, {C}, A)"
 proof -
-  let ?\<M> = "{(C', active)}"
-  and ?\<M>' = "{(C'', passive)}"
+  let ?\<M> = "{(C', Active)}"
+  and ?\<M>' = "{(C'', Passive)}"
   and ?\<N> = "formulas_of (P, {C}, A)"
   have "{C, C''} \<subseteq> fst` (?\<N> \<union> ?\<M>')"
     by simp
@@ -179,9 +162,7 @@ proof -
     by (smt (z3) DiffI Diff_eq_empty_iff assms empty_iff no_labels.Red_F_of_subset)
   then have \<M>_included: " ?\<M> \<subseteq> Red_F_\<G> (?\<N> \<union> ?\<M>')"
     using no_labels_Red_F_imp_Red_F by auto
-  have "passive \<noteq> active"
-    by (simp add: labels_distinct)
-  then have "active_subset ?\<M>' = {}"
+  have "active_subset ?\<M>' = {}"
     using active_subset_def by auto
   then have "(zl_inferences_of T, ?\<N> \<union> ?\<M>) \<leadsto>LGC (zl_inferences_of T, ?\<N> \<union> ?\<M>')"
     using \<M>_included process[of _ _ "?\<M>" _ "?\<M>'"] by auto
@@ -197,20 +178,20 @@ lemma zl_compute_infer_in_lgc:
   shows "zl_state (T \<union> {(LCons \<iota>0 \<iota>s)}, P, {}, A) \<leadsto>LGC zl_state (T \<union> {\<iota>s}, P \<union> {C}, {}, A)"
 proof -
   let ?\<N> = "formulas_of (P, {}, A)"
-  and ?\<M> = "{(C, passive)}"
+  and ?\<M> = "{(C, Passive)}"
 
   have active_subset_of_\<M>: "active_subset ?\<M> = {}"
-    using active_subset_def labels_distinct by auto
+    using active_subset_def by auto
   moreover have "A \<union> {C} \<subseteq> fst ` (?\<N> \<union> ?\<M>)" by auto
   ultimately have "\<iota>0 \<in> no_labels.Red_I (fst ` (?\<N> \<union> ?\<M>))"
     by (meson assms no_labels.empty_ord.Red_I_of_subset subsetD)
   then have compute_one_infer:
     "(zl_inferences_of (T \<union> {\<iota>s}) \<union> {\<iota>0}, formulas_of (P, {}, A)) \<leadsto>LGC
-     (zl_inferences_of (T \<union> {\<iota>s}), formulas_of (P, {}, A) \<union> {(C, passive)})"
+     (zl_inferences_of (T \<union> {\<iota>s}), formulas_of (P, {}, A) \<union> {(C, Passive)})"
     by (metis active_subset_of_\<M> step.compute_infer)
   moreover have "zl_inferences_of (T \<union> {(LCons \<iota>0 \<iota>s)}) = zl_inferences_of (T \<union> {\<iota>s}) \<union> {\<iota>0}"
     by (metis Un_assoc distr_zl_inferences_of_wrt_union flatten)
-  moreover have "formulas_of (P, {}, A) \<union> {(C, passive)} = formulas_of (P \<union> {C}, {}, A)"
+  moreover have "formulas_of (P, {}, A) \<union> {(C, Passive)} = formulas_of (P \<union> {C}, {}, A)"
       using PYA_add_passive_formula by blast
   ultimately show "zl_state (T \<union> {(LCons \<iota>0 \<iota>s)}, P, {}, A) \<leadsto>LGC
              zl_state (T \<union> {\<iota>s}, P \<union> {C}, {}, A)"
@@ -226,17 +207,12 @@ proof -
     by (meson prj_active_subset_of_state)
   then have "zl_inferences_of T' = (no_labels.Inf_between (fst ` (active_subset ?\<N>)) {C})"
     using assms by simp
-
-  also have "y \<noteq> active"
-    using labels_distinct by auto
-
-  then have "(zl_inferences_of T, ?\<N> \<union> {(C, y)}) \<leadsto>LGC
-              (zl_inferences_of T \<union> zl_inferences_of T', ?\<N> \<union> {(C, active)})"
-    using calculation step.schedule_infer by blast
-
-  moreover have "formulas_of (P, {C}, A) = ?\<N> \<union> {(C, y)}"
+  then have "(zl_inferences_of T, ?\<N> \<union> {(C, YY)}) \<leadsto>LGC
+    (zl_inferences_of T \<union> zl_inferences_of T', ?\<N> \<union> {(C, Active)})"
+    using step.schedule_infer by blast
+  moreover have "formulas_of (P, {C}, A) = ?\<N> \<union> {(C, YY)}"
     by auto
-  moreover have "formulas_of (P, {}, A \<union> {C}) = ?\<N> \<union> {(C, active)}"
+  moreover have "formulas_of (P, {}, A \<union> {C}) = ?\<N> \<union> {(C, Active)}"
     by auto
   ultimately have H0: "(zl_inferences_of T, formulas_of (P, {C}, A)) \<leadsto>LGC
     (zl_inferences_of T \<union> zl_inferences_of T', formulas_of (P, {}, A \<union> {C}))"
@@ -247,7 +223,7 @@ qed
 
 lemma zl_delete_orphans_in_lgc:
   assumes " \<forall>n \<in> {n. enat n < llength \<iota>s}. lnth \<iota>s n \<notin> no_labels.Inf_from A"
-  shows "zl_state (T \<union> { \<iota>s }, P, Y, A) \<leadsto>LGC zl_state (T, P, Y, A)"
+  shows "zl_state (T \<union> {\<iota>s}, P, Y, A) \<leadsto>LGC zl_state (T, P, Y, A)"
 proof -
   let ?\<N> = "formulas_of (P, Y, A)"
   and ?\<T>' = "lset \<iota>s"
@@ -262,17 +238,17 @@ proof -
   ultimately have \<iota>s_orphans: "?\<T>' \<inter> no_labels.Inf_from A = {}"
     by auto
 
-  have "fst ` (active_subset ?\<N>) = A"
+  have "fst ` active_subset ?\<N> = A"
     using prj_active_subset_of_state by auto
-  then have \<iota>s_orphans: "?\<T>' \<inter> no_labels.Inf_from (fst ` (active_subset ?\<N>)) = {}"
+  then have \<iota>s_orphans: "?\<T>' \<inter> no_labels.Inf_from (fst ` active_subset ?\<N>) = {}"
     using assms \<iota>s_orphans by auto
 
   have thesis_before_rewriting: "(?\<T> \<union> ?\<T>', ?\<N>) \<leadsto>LGC (?\<T>, ?\<N>)"
     using \<iota>s_orphans step.delete_orphans by presburger
 
-  have "zl_inferences_of (T \<union> { \<iota>s }) = zl_inferences_of T \<union> zl_inferences_of { \<iota>s }"
+  have "zl_inferences_of (T \<union> {\<iota>s}) = zl_inferences_of T \<union> zl_inferences_of {\<iota>s}"
     using distr_zl_inferences_of_wrt_union by auto
-  moreover have "zl_inferences_of (T \<union> { \<iota>s }) = ?\<T> \<union> (lset \<iota>s)"
+  moreover have "zl_inferences_of (T \<union> {\<iota>s}) = ?\<T> \<union> (lset \<iota>s)"
     by auto
   ultimately show ?thesis
     using thesis_before_rewriting zl_state.simps by presburger
